lakefile.lean
@@ -5,6 +5,7 @@ package iris where
   srcDir := "./src/"
 
 require std from git "https://github.com/leanprover/std4" @ "main"
+require Qq from git "https://github.com/gebner/quote4" @ "master"
 
 @[default_target]
 lean_lib iris
