src/Iris/Proofmode.lean
@@ -1,9 +1,7 @@
 import Iris.Proofmode.Classes
 import Iris.Proofmode.Display
-import Iris.Proofmode.Environments
 import Iris.Proofmode.Expr
 import Iris.Proofmode.Instances
 import Iris.Proofmode.Patterns
 import Iris.Proofmode.Tactics
-import Iris.Proofmode.Theorems
 import Iris.Proofmode.UnifHints
