src/Iris/Proofmode/Tactics/Assumption.lean
@@ -1,0 +1,153 @@
+/-
+Copyright (c) 2022 Lars König. All rights reserved.
+Released under Apache 2.0 license as described in the file LICENSE.
+Authors: Lars König, Mario Carneiro
+-/
+import Iris.Proofmode.Tactics.Basic
+import Iris.Proofmode.Tactics.Remove
+
+namespace Iris.Proofmode
+open Lean Elab Tactic Meta Qq BI Std
+
+theorem pure_assumption [BI PROP] {P A Q : PROP} (h_P : ⊢ A)
+    [inst : FromAssumption true A Q] [TCOr (Affine P) (Absorbing Q)] :
+    P ⊢ Q :=
+  have := intuitionistically_emp.2.trans <| (intuitionistically_mono h_P).trans inst.1
+  emp_sep.2.trans <| (sep_mono_l this).trans sep_elim_l
+
+def assumptionLean {prop : Q(Type)} (_bi : Q(BI $prop)) (ehyps goal : Q($prop))
+    (mvar : MVarId) : MetaM Unit := do
+  mvar.withContext do
+    let _ ← synthInstanceQ q(TCOr (Affine $ehyps) (Absorbing $goal))
+    for h in ← getLCtx do
+      let some #[_, _, hh, (P : Q($prop))] := (← whnfR h.type).appM? ``Entails | continue
+      unless (← whnfR hh).isAppOfArity ``BI.emp 2 do continue
+      have h : Q(⊢ $P) := .fvar h.fvarId
+      -- let (name, type) := (h.userName, ← instantiateMVars h.type)
+
+      -- try to solve the goal
+      try
+        let _ ← synthInstanceQ q(FromAssumption true $P $goal)
+        mvar.assign q(pure_assumption (P := $ehyps) (Q := $goal) $h)
+        return
+      catch e => trace[Meta.debug] e.toMessageData; pure ()
+    throwError "no matching hypothesis found"
+
+elab "iassumption_lean" : tactic => do
+  -- retrieve goal mvar declaration
+  let mvar ← getMainGoal
+  mvar.withContext do
+  let g ← instantiateMVars <| ← mvar.getType
+  let some { bi, hyps, goal, .. } := parseIrisGoal? g | throwError "not in proof mode"
+  assumptionLean bi hyps.strip goal mvar
+  replaceMainGoal []
+
+inductive AssumptionFastPath (prop : Q(Type)) (bi : Q(BI $prop)) (Q : Q($prop)) where
+  | absorbing (_ : Q(Absorbing $Q))
+  | biAffine (_ : Q(BIAffine $prop))
+
+variable {prop : Q(Type)} (bi : Q(BI $prop)) (Q : Q($prop))
+  (fastPath : AssumptionFastPath prop bi Q) in
+def assumptionFast (hyps : Hyps prop) : MetaM Q($hyps.strip ⊢ $Q) := do
+  let some ⟨inst, _, out, ty, b, _, pf⟩ ←
+    hyps.removeG bi true fun kind _ ty => try? do
+      let b := match kind with
+      | .intuitionistic => q(true)
+      | .spatial => q(false)
+      synthInstance q(FromAssumption $b $ty $Q)
+    | failure
+  let (_ : Q(FromAssumption $b $ty $Q)) := inst
+  have : $out =Q iprop(□?$b $ty) := ⟨⟩
+  match fastPath with
+  | .absorbing _ =>
+    return q(assumption (Q := $Q) $pf)
+  | .biAffine s =>
+    have : @BIAffine.toBI _ $s =Q $bi := ⟨⟩
+    return q(assumption (Q := $Q) $pf)
+
+inductive AssumptionSlow (prop : Q(Type)) (bi : Q(BI $prop)) (Q e : Q($prop)) where
+  | none
+  | affine (pf : Q(Affine $e))
+  | main (pf : Q($e ⊢ $Q)) (pf : Option Q(Affine $e))
+
+theorem assumption_l [BI PROP] {P Q R : PROP} [Affine Q] (h : P ⊢ R) : P ∗ Q ⊢ R :=
+  sep_elim_l.trans h
+theorem assumption_r [BI PROP] {P Q R : PROP} [Affine P] (h : Q ⊢ R) : P ∗ Q ⊢ R :=
+  sep_elim_r.trans h
+
+variable {prop : Q(Type)} (bi : Q(BI $prop)) (Q : Q($prop)) in
+def assumptionSlow (assume : Bool) :
+    (hyps : Hyps prop) → MetaM (AssumptionSlow prop bi Q hyps.strip)
+  | .emp s =>
+    have : $s =Q emp := ⟨⟩
+    Pure.pure (.affine q(emp_affine))
+  | .hyp _ out kind _ ty => do
+    let b := match kind with
+    | .intuitionistic => q(true)
+    | .spatial => q(false)
+    have : $out =Q iprop(□?$b $ty) := ⟨⟩
+    let fromAssum (_:Unit) := do
+      let _ ← synthInstanceQ q(FromAssumption $b $ty $Q)
+      let inst ← try? (synthInstanceQ q(Affine $out))
+      return .main q(FromAssumption.from_assumption) inst
+    let affine (_:Unit) := return .affine (← synthInstanceQ q(Affine $out))
+    if assume then
+      try fromAssum () catch _ => try affine () catch _ => return .none
+    else
+      try affine () catch _ => try fromAssum () catch _ => return .none
+  | .sep _ s lhs rhs => do
+    let elhs := lhs.strip
+    let erhs := rhs.strip
+    match ← assumptionSlow assume rhs with
+    | .none => return .none
+    | .affine hr =>
+      match ← assumptionSlow assume lhs with
+      | .none => return .none
+      | .affine _ =>
+        have : $s =Q iprop($elhs ∗ $erhs) := ⟨⟩
+        return .affine q(sep_affine ..)
+      | .main lpf (linst : Option Q(Affine $elhs)) =>
+        let linst := linst.map fun hl =>
+          -- FIXME: these haves should not be necessary
+          have elhs := elhs; have erhs := erhs
+          have : Q(Affine $elhs) := hl; have : Q(Affine $erhs) := hr
+          have : $s =Q iprop($elhs ∗ $erhs) := ⟨⟩
+          q(sep_affine $elhs $erhs)
+        have : $s =Q iprop($elhs ∗ $erhs) := ⟨⟩
+        return .main q(assumption_l $lpf) linst
+    | .main rpf rinst =>
+      match ← assumptionSlow false lhs, rinst with
+      | .none, _ | .main _ none, none => return .none
+      | .affine hl, rinst | .main _ (some hl), rinst =>
+        let rinst := rinst.map fun hr =>
+          -- FIXME: these haves should not be necessary
+          have elhs := elhs; have erhs := erhs
+          have : Q(Affine $elhs) := hl; have : Q(Affine $erhs) := hr
+          have : $s =Q iprop($elhs ∗ $erhs) := ⟨⟩
+          q(sep_affine $elhs $erhs)
+        have : $s =Q iprop($elhs ∗ $erhs) := ⟨⟩
+        return .main q(assumption_r $rpf) rinst
+      | .main lpf none, some _ =>
+        have : $s =Q iprop($elhs ∗ $erhs) := ⟨⟩
+        return .main q(assumption_l $lpf) none
+
+elab "iassumption" : tactic => do
+  let mvar ← getMainGoal
+  mvar.withContext do
+  let g ← instantiateMVars <| ← mvar.getType
+  let some { prop, bi, hyps, goal } := parseIrisGoal? g | throwError "not in proof mode"
+
+  let inst : Option (AssumptionFastPath prop bi goal) ← try
+    pure (some (.biAffine (← synthInstanceQ q(BIAffine $prop))))
+  catch _ => try? (AssumptionFastPath.absorbing <$> synthInstanceQ q(Absorbing $goal))
+
+  try
+    let pf ← match inst with
+    | some fastPath => assumptionFast bi goal fastPath hyps
+    | none =>
+      let .main pf _ ← assumptionSlow bi goal true hyps | failure
+      pure pf
+    mvar.assign pf
+  catch _ =>
+    assumptionLean bi hyps.strip goal mvar
+  replaceMainGoal []
