src/Iris/Proofmode/Tactics/Basic.lean
@@ -1,0 +1,53 @@
+/-
+Copyright (c) 2022 Lars König. All rights reserved.
+Released under Apache 2.0 license as described in the file LICENSE.
+Authors: Lars König, Mario Carneiro
+-/
+import Iris.Proofmode.Expr
+import Iris.Proofmode.Classes
+
+namespace Iris.Proofmode
+open Lean Elab.Tactic Meta Qq BI Std
+
+def istart (mvar : MVarId) : MetaM (MVarId × IrisGoal) := mvar.withContext do
+  -- parse goal
+  let goal ← instantiateMVars <| ← mvar.getType
+
+  -- check if already in proof mode
+  if let some irisGoal := parseIrisGoal? goal then
+    return (mvar, irisGoal)
+
+  let some goal ← checkTypeQ goal q(Prop)
+    | throwError "type mismatch\n{← mkHasTypeButIsExpectedMsg (← inferType goal) q(Prop)}"
+  let prop ← mkFreshExprMVarQ q(Type)
+  let P ← mkFreshExprMVarQ q($prop)
+  let bi ← mkFreshExprMVarQ q(BI $prop)
+  let _ ← synthInstanceQ q(Proofmode.AsEmpValid2 $goal $P)
+
+  let irisGoal := { prop, bi, hyps := .mkEmp bi, goal := P }
+  let subgoal : Quoted q(⊢ $P) ←
+    mkFreshExprSyntheticOpaqueMVar (IrisGoal.toExpr irisGoal) (← mvar.getTag)
+  mvar.assign q(Proofmode.as_emp_valid_2 $goal $subgoal)
+  pure (subgoal.mvarId!, irisGoal)
+
+elab "istart" : tactic => do
+  let (mvar, _) ← istart (← getMainGoal)
+  replaceMainGoal [mvar]
+
+elab "istop" : tactic => do
+  -- parse goal
+  let mvar ← getMainGoal
+  mvar.withContext do
+  let goal ← instantiateMVars <| ← mvar.getType
+
+  -- check if already in proof mode
+  let some irisGoal := parseIrisGoal? goal | throwError "not in proof mode"
+  mvar.setType irisGoal.strip
+
+theorem assumption [BI PROP] {p : Bool} {P P' A Q : PROP} [inst : FromAssumption p A Q]
+  [TCOr (Affine P') (Absorbing Q)] (h : P ⊣⊢ P' ∗ □?p A) : P ⊢ Q :=
+  h.1.trans <| (sep_mono_r inst.1).trans sep_elim_r
+
+def getFreshName : Option Name → CoreM Name
+  | none => mkFreshUserName `x
+  | some name => pure name
