src/Iris/Proofmode/Tactics/ExFalso.lean
@@ -1,0 +1,23 @@
+/-
+Copyright (c) 2022 Lars König. All rights reserved.
+Released under Apache 2.0 license as described in the file LICENSE.
+Authors: Lars König, Mario Carneiro
+-/
+import Iris.Proofmode.Expr
+
+namespace Iris.Proofmode
+open Lean Elab.Tactic Meta Qq BI
+
+theorem exfalso [BI PROP] {P Q : PROP} (h : P ⊢ False) : P ⊢ Q := h.trans false_elim
+
+elab "iexfalso" : tactic => do
+  let mvar ← getMainGoal
+  mvar.withContext do
+  let g ← instantiateMVars <| ← mvar.getType
+  let some { prop, bi, hyps, goal } := parseIrisGoal? g | throwError "not in proof mode"
+
+  have ehyps := hyps.strip
+  let m : Q($ehyps ⊢ False) ← mkFreshExprSyntheticOpaqueMVar <|
+    IrisGoal.toExpr { prop, bi, hyps, goal := q(iprop(False)) }
+  mvar.assign q(exfalso (Q := $goal) $m)
+  replaceMainGoal [m.mvarId!]
