src/Iris/Proofmode/Tactics/Exact.lean
@@ -1,0 +1,29 @@
+/-
+Copyright (c) 2022 Lars König. All rights reserved.
+Released under Apache 2.0 license as described in the file LICENSE.
+Authors: Lars König, Mario Carneiro
+-/
+import Iris.Proofmode.Tactics.Basic
+import Iris.Proofmode.Tactics.Remove
+
+namespace Iris.Proofmode
+open Lean Elab Tactic Meta Qq BI Std
+
+elab "iexact" colGt hyp:ident : tactic => do
+  -- parse syntax
+  let name := hyp.getId
+  if name.isAnonymous then
+    throwUnsupportedSyntax
+
+  -- find hypothesis index
+  let mvar ← getMainGoal
+  mvar.withContext do
+  let g ← instantiateMVars <| ← mvar.getType
+  let some { bi, hyps, goal, .. } := parseIrisGoal? g | throwError "not in proof mode"
+  let some ⟨hyps', _, out, p, _, pf⟩ := hyps.remove bi true name | throwError "unknown hypothesis"
+
+  let _ ← synthInstanceQ q(FromAssumption $p $out $goal)
+  let _ ← synthInstanceQ q(TCOr (Affine $hyps'.strip) (Absorbing $goal))
+
+  mvar.assign q(assumption (Q := $goal) $pf)
+  replaceMainGoal []
