src/Iris/Proofmode/Tactics/Exists.lean
@@ -1,0 +1,30 @@
+/-
+Copyright (c) 2022 Lars König. All rights reserved.
+Released under Apache 2.0 license as described in the file LICENSE.
+Authors: Lars König, Mario Carneiro
+-/
+import Iris.Proofmode.Tactics.Basic
+
+namespace Iris.Proofmode
+open Lean Elab Tactic Meta Qq BI
+
+theorem exists_intro' [BI PROP] {Φ : α → PROP} {P Q : PROP} [inst : FromExists Q Φ]
+    (a : α) (h : P ⊢ Φ a) : P ⊢ Q :=
+  h.trans <| (exists_intro a).trans inst.1
+
+elab "iexists" x:term : tactic => do
+  -- resolve existential quantifier with the given argument
+
+  let (mvar, { prop, bi, hyps, goal }) ← istart (← getMainGoal)
+  mvar.withContext do
+  have ehyps := hyps.strip
+
+  let α ← mkFreshExprMVarQ q(Type)
+  let Φ ← mkFreshExprMVarQ q($α → $prop)
+  let _ ← synthInstanceQ q(FromExists $goal $Φ)
+  let x ← elabTermEnsuringTypeQ (u := .succ .zero) x α
+  let m : Quoted q($ehyps ⊢ $Φ $x) ← mkFreshExprSyntheticOpaqueMVar <|
+    IrisGoal.toExpr { prop, bi, hyps, goal := Expr.headBeta q($Φ $x) }
+
+  mvar.assign q(exists_intro' (Q := $goal) $x $m)
+  replaceMainGoal [m.mvarId!]
