src/Iris/Proofmode/Tactics/Intro.lean
@@ -1,0 +1,113 @@
+/-
+Copyright (c) 2022 Lars König. All rights reserved.
+Released under Apache 2.0 license as described in the file LICENSE.
+Authors: Lars König, Mario Carneiro
+-/
+import Iris.Proofmode.Tactics.Cases
+
+namespace Iris.Proofmode
+open Lean Elab Tactic Meta Qq BI Std
+
+theorem imp_intro_drop [BI PROP] {P Q A1 A2 : PROP} [inst : FromImp Q A1 A2] (h : P ⊢ A2) : P ⊢ Q :=
+  BI.imp_intro (and_elim_l' h) |>.trans inst.1
+
+theorem from_forall_intro [BI PROP] {P Q : PROP} {Φ : α → PROP} [inst : FromForall Q Φ]
+    (h : ∀ a, P ⊢ Φ a) : P ⊢ Q :=
+  (forall_intro h).trans inst.1
+
+theorem imp_intro_intuitionistic [BI PROP] {P Q A1 A2 B : PROP}
+    [FromImp Q A1 A2] [inst : IntoPersistently false A1 B] (h : P ∗ □ B ⊢ A2) : P ⊢ Q := by
+  refine BI.imp_intro ?_ |>.trans from_imp
+  exact (and_mono_r inst.1).trans <| persistently_and_intuitionistically_sep_r.1.trans h
+
+theorem wand_intro_intuitionistic [BI PROP] {P Q A1 A2 B : PROP}
+    [FromWand Q A1 A2] [inst : IntoPersistently false A1 B] [or : TCOr (Affine A1) (Absorbing A2)]
+    (h : P ∗ □ B ⊢ A2) : P ⊢ Q := by
+  refine (wand_intro ?_).trans from_wand
+  exact match or with
+  | TCOr.l => (sep_mono_r <| (affine_affinely A1).2.trans (affinely_mono inst.1)).trans h
+  | TCOr.r => (sep_mono_r <| inst.1.trans absorbingly_intuitionistically.2).trans <|
+      absorbingly_sep_r.1.trans <| (absorbingly_mono h).trans absorbing
+
+theorem imp_intro_spatial [BI PROP] {P Q A1 A2 B : PROP}
+    [FromImp Q A1 A2] [inst : FromAffinely B A1] [or : TCOr (Persistent A1) (Intuitionistic P)]
+    (h : P ∗ B ⊢ A2) : P ⊢ Q := by
+  refine (BI.imp_intro ?_).trans from_imp
+  refine Entails.trans ?_ <| (sep_mono_r inst.1).trans h
+  exact match or with
+  | TCOr.l => persistent_and_affinely_sep_r_1
+  | TCOr.r (u := u) =>
+    (and_mono_l u.1).trans <| affinely_and_lr.1.trans <|
+    persistently_and_intuitionistically_sep_l.1.trans <| sep_mono_l intuitionistically_elim
+
+theorem wand_intro_spatial [BI PROP] {P Q A1 A2 : PROP}
+    [FromWand Q A1 A2] (h : P ∗ A1 ⊢ A2) : P ⊢ Q := (wand_intro h).trans from_wand
+
+variable {prop : Q(Type)} (bi : Q(BI $prop)) in
+partial def iIntroCore
+    (hyps : Hyps prop) (Q : Q($prop)) (pats : List iCasesPat)
+    (k : (hyps : Hyps prop) → (Q : Q($prop)) → MetaM Q($hyps.strip ⊢ $Q)) :
+    MetaM (Q($hyps.strip ⊢ $Q)) := do
+  match pats with
+  | [] => k hyps Q
+  | pat :: pats =>
+    let A1 ← mkFreshExprMVarQ q($prop)
+    let A2 ← mkFreshExprMVarQ q($prop)
+    let fromImp ← try? (α := Q(FromImp $Q $A1 $A2)) do
+      synthInstanceQ q(FromImp $Q $A1 $A2)
+    if let (.clear, some _) := (pat, fromImp) then
+      let pf ← iIntroCore hyps A2 pats k
+      return q(imp_intro_drop (Q := $Q) $pf)
+    else
+    let alres ← try? (α := _ × (α : Q(Type)) × (Φ : Q($α → $prop)) × Q(FromForall $Q $Φ)) do
+      let .one n := pat | failure
+      let α ← mkFreshExprMVarQ q(Type)
+      let Φ ← mkFreshExprMVarQ q($α → $prop)
+      Pure.pure ⟨n, α, Φ, ← synthInstanceQ q(FromForall $Q $Φ)⟩
+    if let some ⟨n, α, Φ, _⟩ := alres then
+      withLocalDeclDQ (← getFreshName n) α fun x => do
+        have B : Q($prop) := Expr.headBeta q($Φ $x)
+        have : $B =Q $Φ $x := ⟨⟩
+        let pf : Q(∀ x, $hyps.strip ⊢ $Φ x) ← mkLambdaFVars #[x] <|← iIntroCore hyps B pats k
+        return q(from_forall_intro (Q := $Q) $pf)
+    else
+    let B ← mkFreshExprMVarQ q($prop)
+    match pat, fromImp with
+    | .intuitionistic pat, some _ =>
+      let _ ← synthInstanceQ q(IntoPersistently false $A1 $B)
+      let pf ← iCasesCore bi hyps A2 q(true) q(iprop(□ $B)) B ⟨⟩ pat (iIntroCore · A2 pats k)
+      return q(imp_intro_intuitionistic (Q := $Q) $pf)
+    | .intuitionistic pat, none =>
+      let _ ← synthInstanceQ q(FromWand $Q $A1 $A2)
+      let _ ← synthInstanceQ q(IntoPersistently false $A1 $B)
+      let _ ← synthInstanceQ q(TCOr (Affine $A1) (Absorbing $A2))
+      let pf ← iCasesCore bi hyps A2 q(true) q(iprop(□ $B)) B ⟨⟩ pat (iIntroCore · A2 pats k)
+      return q(wand_intro_intuitionistic (Q := $Q) $pf)
+    | _, some _ =>
+      let _ ← synthInstanceQ q(FromAffinely $B $A1)
+      let _ ← synthInstanceQ q(TCOr (Persistent $A1) (Intuitionistic $hyps.strip))
+      let pf ← iCasesCore bi hyps A2 q(false) B B ⟨⟩ pat (iIntroCore · A2 pats k)
+      return q(imp_intro_spatial (Q := $Q) $pf)
+    | _, none =>
+      let _ ← synthInstanceQ q(FromWand $Q $A1 $A2)
+      let pf ← iCasesCore bi hyps A2 q(false) A1 A1 ⟨⟩ pat (iIntroCore · A2 pats k)
+      return q(wand_intro_spatial (Q := $Q) $pf)
+
+
+elab "iintro" pats:(colGt icasesPat)* : tactic => do
+  -- parse syntax
+  let pats ← liftMacroM <| pats.mapM <| iCasesPat.parse
+
+  let (mvar, { prop, bi, hyps, goal }) ← istart (← getMainGoal)
+  mvar.withContext do
+
+  -- process patterns
+  let goals ← IO.mkRef #[]
+  let pf ← iIntroCore bi hyps goal pats.toList fun hyps goal => do
+    let m : Q($hyps.strip ⊢ $goal) ← mkFreshExprSyntheticOpaqueMVar <|
+      IrisGoal.toExpr { prop, bi, hyps, goal }
+    goals.modify (·.push m.mvarId!)
+    pure m
+
+  mvar.assign pf
+  replaceMainGoal (← goals.get).toList
