src/Iris/Proofmode/Tactics/Move.lean
@@ -1,0 +1,137 @@
+/-
+Copyright (c) 2022 Lars König. All rights reserved.
+Released under Apache 2.0 license as described in the file LICENSE.
+Authors: Lars König, Mario Carneiro
+-/
+import Iris.Proofmode.Expr
+import Iris.Proofmode.Classes
+
+namespace Iris.Proofmode
+open Lean Elab Tactic Meta Qq BI Std
+
+def Replaces [BI PROP] (K A B : PROP) := (B -∗ K) ⊢ (A -∗ K)
+
+theorem replaces_r [BI PROP] {K P Q Q' : PROP} (h : Replaces K Q Q') :
+    Replaces K iprop(P ∗ Q) iprop(P ∗ Q') :=
+  wand_intro <| sep_assoc.2.trans <| wand_elim <|
+  (wand_intro <| sep_assoc.1.trans wand_elim_l).trans h
+
+theorem replaces_l [BI PROP] {K P P' Q : PROP} (h : Replaces K P P') :
+    Replaces K iprop(P ∗ Q) iprop(P' ∗ Q) :=
+  (wand_mono_l sep_comm.1).trans <| (replaces_r h).trans (wand_mono_l sep_comm.1)
+
+theorem Replaces.apply [BI PROP] {P P' Q : PROP}
+    (h : Replaces Q P P') (h_entails : P' ⊢ Q) : P ⊢ Q :=
+  wand_entails <| (entails_wand h_entails).trans h
+
+inductive ReplaceHyp (prop : Q(Type)) (bi : Q(BI $prop)) (Q : Q($prop)) where
+  | none
+  | unchanged (hyps' : Hyps prop)
+  | main (hyps' : Hyps prop) (e e' : Q($prop)) (pf : Q(Replaces $Q $e $e'))
+
+variable [Monad m] {prop : Q(Type)} (bi : Q(BI $prop)) (Q : Q($prop))
+  (name : Name) (repl : HypothesisKind → Q($prop) → MetaM (ReplaceHyp prop bi Q)) in
+def Hyps.replace : Hyps prop → MetaM (ReplaceHyp prop bi Q)
+  | .emp _ => pure .none
+  | .hyp _ _ kind name' ty => do
+    if name == name' then
+      let res ← repl kind ty
+      if let .main hyps' e e' _ := res then
+        let e' ← instantiateMVarsQ e'
+        if e == e' then
+          return .unchanged hyps'
+      return res
+    else return .none
+  | .sep _ _ lhs rhs => do
+    match ← rhs.replace with
+    | .unchanged rhs' => return .unchanged (.mkSep bi lhs rhs')
+    | .main rhs' erhs' e' pf =>
+      have elhs := lhs.strip
+      let hyps' := .mkSep bi lhs rhs'
+      return .main hyps' q(iprop($elhs ∗ $erhs')) q(iprop($elhs ∗ $e')) q(replaces_r $pf)
+    | .none => match ← lhs.replace with
+      | .unchanged lhs' => return .unchanged (.mkSep bi lhs' rhs)
+      | .main lhs' elhs' e' pf =>
+        have erhs := rhs.strip
+        let hyps' := .mkSep bi lhs' rhs
+        return .main hyps' q(iprop($elhs' ∗ $erhs)) q(iprop($e' ∗ $erhs)) q(replaces_l $pf)
+      | .none => pure .none
+
+theorem to_persistent_spatial [BI PROP] {P P' Q : PROP}
+    [hP : IntoPersistently false P P'] [or : TCOr (Affine P) (Absorbing Q)] :
+    Replaces Q P iprop(□ P') :=
+  match or with
+  | TCOr.l => wand_mono_l <| (affine_affinely P).2.trans (affinely_mono hP.1)
+  | TCOr.r =>
+    wand_intro <| (sep_mono_r <| hP.1.trans absorbingly_intuitionistically.2).trans <|
+    absorbingly_sep_r.1.trans <| (absorbingly_mono wand_elim_l).trans absorbing
+
+theorem to_persistent_intuitionistic [BI PROP] {P P' Q : PROP}
+    [hP : IntoPersistently true P P'] : Replaces Q iprop(□ P) iprop(□ P') :=
+  wand_mono_l <| affinely_mono hP.1
+
+elab "iintuitionistic" colGt hyp:ident : tactic => do
+  -- parse syntax
+  let name := hyp.getId
+  if name.isAnonymous then
+    throwUnsupportedSyntax
+
+  let mvar ← getMainGoal
+  mvar.withContext do
+  let g ← instantiateMVars <| ← mvar.getType
+  let some { prop, bi, hyps, goal } := parseIrisGoal? g | throwError "not in proof mode"
+
+  match ← hyps.replace bi goal name fun kind ty => do
+    let P' ← mkFreshExprMVarQ prop
+    match kind with
+    | .intuitionistic =>
+      let _ ← synthInstanceQ q(IntoPersistently true $ty $P')
+      return .main (.mkHyp bi .intuitionistic name P')
+        q(iprop(□ $ty)) q(iprop(□ $P')) q(to_persistent_intuitionistic)
+    | .spatial =>
+      let _ ← synthInstanceQ q(IntoPersistently false $ty $P')
+      let _ ← synthInstanceQ q(TCOr (Affine $ty) (Absorbing $goal))
+      return .main (.mkHyp bi .intuitionistic name P') ty q(iprop(□ $P')) q(to_persistent_spatial)
+  with
+  | .none => throwError "unknown hypothesis"
+  | .unchanged hyps' =>
+    mvar.setType <| IrisGoal.toExpr { prop, bi, hyps := hyps', goal }
+  | .main hyps' _e e' pf =>
+    let m : Q($e' ⊢ $goal) ← mkFreshExprSyntheticOpaqueMVar <|
+      IrisGoal.toExpr { prop, bi, hyps := hyps', goal }
+    mvar.assign q(Replaces.apply $pf $m)
+    replaceMainGoal [m.mvarId!]
+
+theorem from_affine [BI PROP] {p : Bool} {P P' Q : PROP} [hP : FromAffinely P' P p] :
+    Replaces Q iprop(□?p P) P' :=
+  wand_mono_l <| affinelyIf_of_intuitionisticallyIf.trans hP.1
+
+elab "ispatial" colGt hyp:ident : tactic => do
+  -- parse syntax
+  let name := hyp.getId
+  if name.isAnonymous then
+    throwUnsupportedSyntax
+
+  let mvar ← getMainGoal
+  mvar.withContext do
+  let g ← instantiateMVars <| ← mvar.getType
+  let some { prop, bi, hyps, goal } := parseIrisGoal? g | throwError "not in proof mode"
+
+  match ← hyps.replace bi goal name fun kind ty => do
+    let P' ← mkFreshExprMVarQ prop
+    match kind with
+    | .intuitionistic =>
+      let _ ← synthInstanceQ q(FromAffinely $P' $ty true)
+      return .main (.mkHyp bi .spatial name P') q(iprop(□ $ty)) P' q(from_affine (p := true))
+    | .spatial =>
+      let _ ← synthInstanceQ q(FromAffinely $P' $ty false)
+      return .main (.mkHyp bi .spatial name P') ty P' q(from_affine (p := false))
+  with
+  | .none => throwError "unknown hypothesis"
+  | .unchanged hyps' =>
+    mvar.setType <| IrisGoal.toExpr { prop, bi, hyps := hyps', goal }
+  | .main hyps' _e e' pf =>
+    let m : Q($e' ⊢ $goal) ← mkFreshExprSyntheticOpaqueMVar <|
+      IrisGoal.toExpr { prop, bi, hyps := hyps', goal }
+    mvar.assign q(Replaces.apply $pf $m)
+    replaceMainGoal [m.mvarId!]
