src/Iris/Proofmode/Tactics/Rename.lean
@@ -1,63 +1,40 @@
 /-
 Copyright (c) 2022 Lars König. All rights reserved.
 Released under Apache 2.0 license as described in the file LICENSE.
-Authors: Lars König
+Authors: Lars König, Mario Carneiro
 -/
+import Iris.BI
 import Iris.Proofmode.Expr
+import Iris.Proofmode.Classes
+import Iris.Std
+import Lean.Elab
 
-import Lean.Elab.Tactic
+namespace Iris.Proofmode
+open Lean Elab Tactic Qq
 
-namespace Iris.Proofmode.Internal
-open Lean Lean.Elab.Tactic Lean.Meta
+variable (old new : Name) {prop : Q(Type)} (bi : Q(BI $prop)) in
+def Hyps.rename : Hyps prop → Option (Hyps prop)
+  | .emp _ => none
+  | .sep _ _ lhs rhs =>
+    match rhs.rename with
+    | some rhs' => some (.mkSep bi lhs rhs')
+    | none => match lhs.rename with
+      | some lhs' => some (.mkSep bi lhs' rhs)
+      | none => none
+  | .hyp _ _ kind name ty => if old == name then some (Hyps.mkHyp bi kind new ty) else none
 
-def irenameCore (hypIndex : HypothesisIndex) (name : Name) : TacticM Unit := do
-  -- parse goal
-  let goal ← getMainGoal
-  let expr ← instantiateMVars <| ← goal.getType
+elab "irename" colGt nameFrom:ident " => " colGt nameTo:ident : tactic => do
+  -- parse syntax
+  if nameFrom.getId.isAnonymous || nameTo.getId.isAnonymous then
+    throwUnsupportedSyntax
 
-  let some (Γₚ, Γₛ, _) ← extractEnvsEntails? expr
-    | throwError "not in proof mode"
+  -- find hypothesis index
+  let mvar ← getMainGoal
+  mvar.withContext do
+  let g ← instantiateMVars <| ← mvar.getType
+  let some { prop, bi, hyps, goal } := parseIrisGoal? g | throwError "not in proof mode"
 
-  -- retrieve goal mvar declaration
-  let some decl := (← getMCtx).findDecl? goal
-    | throwError "ill-formed proof environment"
+  let some hyps' := hyps.rename nameFrom.getId nameTo.getId bi
+    | throwError "unknown hypothesis"
 
-  let modifyHypothesis (Γ : Expr) (idx : Nat) : TacticM Expr := do
-    -- find hypothesis
-    let some h ← EnvExpr.get? Γ idx
-      | throwError "invalid index or ill-formed proof environment"
-
-    -- check for unique (or equal) hypothesis name
-    let nameFrom? := h.getMDataName?
-    if nameFrom? |>.map (· != name) |>.getD true then
-      if ← [Γₚ, Γₛ].anyM fun Γ =>
-        return (← EnvExpr.any? Γ (·.getMDataName?.isEqSome name)) matches some true
-      then
-        throwError "name is already used for another hypothesis"
-
-      if decl.lctx.any (·.userName == name) then
-        throwError "name is already used in the Lean context"
-
-    -- rename hypothesis
-    let h := h.setMDataName? name
-
-    -- re-insert hypothesis
-    let some Γ ← EnvExpr.set? Γ h idx
-      | throwError "invalid index or ill-formed proof environment"
-
-    return Γ
-
-  -- modify environment
-  let (Γₚ, Γₛ) ← match hypIndex with
-    | ⟨.intuitionistic, index, _⟩ => do
-      pure (← modifyHypothesis Γₚ index, Γₛ)
-    | ⟨.spatial, index, _⟩ => do
-      pure (Γₚ, ← modifyHypothesis Γₛ index)
-
-  -- update goal
-  let some expr ← modifyEnvsEntails? expr Γₚ Γₛ none
-    | throwError "ill-formed proof environment"
-
-  goal.setType expr
-
-end Iris.Proofmode.Internal
+  mvar.setType (IrisGoal.toExpr { prop, bi, hyps := hyps', goal })
