src/Iris/Proofmode/Tactics/Split.lean
@@ -1,0 +1,132 @@
+/-
+Copyright (c) 2022 Lars König. All rights reserved.
+Released under Apache 2.0 license as described in the file LICENSE.
+Authors: Lars König, Mario Carneiro
+-/
+import Iris.Proofmode.Tactics.Basic
+import Iris.Proofmode.Tactics.Remove
+
+namespace Iris.Proofmode
+open Lean Elab Tactic Meta Qq BI
+
+theorem from_and_intro [BI PROP] {P Q A1 A2 : PROP} [inst : FromAnd Q A1 A2]
+    (h1 : P ⊢ A1) (h2 : P ⊢ A2) : P ⊢ Q :=
+  (and_intro h1 h2).trans inst.1
+
+elab "isplit" : tactic => do
+  let (mvar, { prop, bi, hyps, goal }) ← istart (← getMainGoal)
+  mvar.withContext do
+
+  have ehyps := hyps.strip
+  let A1 ← mkFreshExprMVarQ prop
+  let A2 ← mkFreshExprMVarQ prop
+  let _ ← synthInstanceQ q(FromAnd $goal $A1 $A2)
+  let m1 : Q($ehyps ⊢ $A1) ← mkFreshExprSyntheticOpaqueMVar <|
+    IrisGoal.toExpr { prop, bi, hyps, goal := A1 }
+  let m2 : Q($ehyps ⊢ $A2) ← mkFreshExprSyntheticOpaqueMVar <|
+    IrisGoal.toExpr { prop, bi, hyps, goal := A2 }
+  mvar.assign q(from_and_intro (Q := $goal) $m1 $m2)
+  replaceMainGoal [m1.mvarId!, m2.mvarId!]
+
+
+theorem split_es [BI PROP] {Q Q1 Q2 : PROP} (h : Q ⊣⊢ Q1 ∗ Q2) : emp ∗ Q ⊣⊢ Q1 ∗ Q2 :=
+  emp_sep.trans h
+theorem split_ls [BI PROP] {P Q Q1 Q2 : PROP} (h : Q ⊣⊢ Q1 ∗ Q2) : P ∗ Q ⊣⊢ (P ∗ Q1) ∗ Q2 :=
+  (sep_congr_r h).trans sep_assoc.symm
+theorem split_rs [BI PROP] {P Q Q1 Q2 : PROP} (h : Q ⊣⊢ Q1 ∗ Q2) : P ∗ Q ⊣⊢ Q1 ∗ (P ∗ Q2) :=
+  (sep_congr_r h).trans sep_left_comm
+theorem split_se [BI PROP] {P P1 P2 : PROP} (h : P ⊣⊢ P1 ∗ P2) : P ∗ emp ⊣⊢ P1 ∗ P2 :=
+  sep_emp.trans h
+theorem split_sl [BI PROP] {P Q P1 P2 : PROP} (h : P ⊣⊢ P1 ∗ P2) : P ∗ Q ⊣⊢ (P1 ∗ Q) ∗ P2 :=
+  (sep_congr_l h).trans sep_right_comm
+theorem split_sr [BI PROP] {P Q P1 P2 : PROP} (h : P ⊣⊢ P1 ∗ P2) : P ∗ Q ⊣⊢ P1 ∗ (P2 ∗ Q) :=
+  (sep_congr_l h).trans sep_assoc
+theorem split_ss [BI PROP] {P Q P1 P2 Q1 Q2 : PROP}
+    (h1 : P ⊣⊢ P1 ∗ P2) (h2 : Q ⊣⊢ Q1 ∗ Q2) : P ∗ Q ⊣⊢ (P1 ∗ Q1) ∗ (P2 ∗ Q2) :=
+  (sep_congr h1 h2).trans sep_sep_sep_comm
+
+inductive SplitResult (prop : Q(Type)) (bi : Q(BI $prop)) (e : Q($prop)) where
+  | emp (_ : $e =Q BI.emp)
+  | left
+  | right
+  | split (lhs rhs : Hyps prop) (elhs erhs : Q($prop)) (pf : Q($e ⊣⊢ $elhs ∗ $erhs))
+
+variable (prop : Q(Type)) (bi : Q(BI $prop)) (toRight : Name → Bool) in
+def Hyps.splitCore : (h : Hyps prop) → SplitResult prop bi h.strip
+  | .emp _ => .emp ⟨⟩
+  | h@(.hyp _ ehyp .intuitionistic _ ty) =>
+    have : $ehyp =Q iprop(□ $ty) := ⟨⟩
+    .split h h ehyp ehyp q(intuitionistically_sep_dup)
+  | .hyp _ _ .spatial name _ => if toRight name then .right else .left
+  | .sep _ ehyp lhs rhs =>
+    let resl := lhs.splitCore; let elhs := lhs.strip
+    let resr := rhs.splitCore; let erhs := rhs.strip
+    have : iprop($elhs ∗ $erhs) =Q $ehyp := ⟨⟩
+    match resl, resr with
+    | .emp _, .emp _ | .left, .emp _ | .emp _, .left | .left, .left => .left
+    | .right, .emp _ | .emp _, .right | .right, .right => .right
+    | .left, .right => .split lhs rhs elhs erhs q(.rfl)
+    | .right, .left => .split rhs lhs erhs elhs q(sep_comm)
+    | .emp _, .split r1 r2 er1 er2 rpf => .split r1 r2 er1 er2 q(split_es $rpf)
+    | .left, .split r1 r2 er1 er2 rpf =>
+      .split (lhs.mkSep bi r1) r2 q(iprop($elhs ∗ $er1)) er2 q(split_ls $rpf)
+    | .right, .split r1 r2 er1 er2 rpf =>
+      .split r1 (lhs.mkSep bi r2) er1 q(iprop($elhs ∗ $er2)) q(split_rs $rpf)
+    | .split l1 l2 el1 el2 lpf, .emp _ => .split l1 l2 el1 el2 q(split_se $lpf)
+    | .split l1 l2 el1 el2 lpf, .left =>
+      .split (l1.mkSep bi rhs) l2 q(iprop($el1 ∗ $erhs)) el2 q(split_sl $lpf)
+    | .split l1 l2 el1 el2 lpf, .right =>
+      .split l1 (l2.mkSep bi rhs) el1 q(iprop($el2 ∗ $erhs)) q(split_sr $lpf)
+    | .split l1 l2 el1 el2 lpf, .split r1 r2 er1 er2 rpf =>
+      .split (l1.mkSep bi r1) (l2.mkSep bi r2) q(iprop($el1 ∗ $er1)) q(iprop($el2 ∗ $er2))
+        q(split_ss $lpf $rpf)
+
+def Hyps.split (prop : Q(Type)) (bi : Q(BI $prop)) (toRight : Name → Bool) (hyps : Hyps prop) :
+    (_lhs _rhs : Hyps prop) × (elhs erhs : Q($prop)) × Q($(hyps.strip) ⊣⊢ $elhs ∗ $erhs) :=
+  let ehyps := hyps.strip
+  match hyps.splitCore prop bi toRight with
+  | .emp _ => ⟨hyps, hyps, ehyps, ehyps, q(sep_emp_rev)⟩
+  | .left => ⟨hyps, .mkEmp bi, ehyps, q(BI.emp), q(sep_emp_rev)⟩
+  | .right => ⟨.mkEmp bi, hyps, q(BI.emp), ehyps, q(emp_sep_rev)⟩
+  | .split lhs rhs el er pf => ⟨lhs, rhs, el, er, pf⟩
+
+theorem sep_split [BI PROP] {P P1 P2 Q Q1 Q2 : PROP} [inst : FromSep Q Q1 Q2]
+    (h : P ⊣⊢ P1 ∗ P2) (h1 : P1 ⊢ Q1) (h2 : P2 ⊢ Q2) : P ⊢ Q :=
+  h.1.trans <| (sep_mono h1 h2).trans inst.1
+
+declare_syntax_cat splitSide
+syntax "l" : splitSide
+syntax "r" : splitSide
+
+elab "isplit" side:splitSide "[" hyps:ident,* "]" : tactic => do
+  -- parse syntax
+  let splitRight ← match side with
+    | `(splitSide| l) => pure false
+    | `(splitSide| r) => pure true
+    | _  => throwUnsupportedSyntax
+  let names ← hyps.getElems.mapM fun name => do
+    let name := name.getId
+    if name.isAnonymous then
+      throwUnsupportedSyntax
+    pure name
+
+  -- extract environment
+  let (mvar, { prop, bi, hyps, goal }) ← istart (← getMainGoal)
+  mvar.withContext do
+
+  let Q1 ← mkFreshExprMVarQ prop
+  let Q2 ← mkFreshExprMVarQ prop
+  let _ ← synthInstanceQ q(FromSep $goal $Q1 $Q2)
+
+  -- split conjunction
+  let ⟨lhs, rhs, el, er, pf⟩ := hyps.split prop bi (names.contains · == splitRight)
+
+  let m1 : Q($el ⊢ $Q1) ← mkFreshExprSyntheticOpaqueMVar <|
+    IrisGoal.toExpr { prop, bi, hyps := lhs, goal := Q1 }
+  let m2 : Q($er ⊢ $Q2) ← mkFreshExprSyntheticOpaqueMVar <|
+    IrisGoal.toExpr { prop, bi, hyps := rhs, goal := Q2 }
+  mvar.assign q(sep_split (Q := $goal) $pf $m1 $m2)
+  replaceMainGoal [m1.mvarId!, m2.mvarId!]
+
+macro "isplit" &"l" : tactic => `(tactic| isplit r [])
+macro "isplit" &"r" : tactic => `(tactic| isplit l [])
