src/Iris/Std.lean
@@ -5,3 +5,4 @@ import Iris.Std.Prod
 import Iris.Std.Rewrite
 import Iris.Std.Tactic
 import Iris.Std.TC
+import Iris.Std.Try
