src/Iris/Std/Try.lean
@@ -1,0 +1,8 @@
+/-
+Copyright (c) 2023 Mario Carneiro. All rights reserved.
+Released under Apache 2.0 license as described in the file LICENSE.
+Authors: Mario Carneiro
+-/
+
+def try? [Monad m] [MonadExcept ε m] (x : m α) : m (Option α) :=
+  try pure (some (← x)) catch _ => pure none
